specs and boolean with proofs for a variant of ACT state checker

ActVarRulesBoolScript.sml
@@ -61,7 +61,7 @@ val ELECT_dec = Define `
      (ELECT_dec ((qu,st,l): params)
            (NonFinal (ba, t, p, bl, bl2, e, h))
            (NonFinal (ba', t', p', bl', bl2', e',h')) <=>
-                   (ELECT_Auxiliary_dec (qu,st,l) ba t p p' bl bl' e e' h h')
+                   (ELECT_Auxiliary_dec (qu,st,l) ba t p p' bl bl' e e' h h' (DROP (LENGTH bl) bl'))
                 /\ (bl2 = bl2') /\ (bl2 = [])
                 /\ (ba = []) /\ (ba' = [])
                 /\ (t = t')
@@ -71,6 +71,12 @@ val ELECT_dec = Define `
 
 
 val TRANSFER_EXCLUDED_dec_def = Define `
+    TRANSFER_EXCLUDED_dec (qu,st,l) j1 j2  <=> TRANSFER_EXCLUDED_Auxiliary_dec (qu,st,l) j1 j2`;
+
+
+
+(*
+val TRANSFER_EXCLUDED_dec_def = Define `
     (TRANSFER_EXCLUDED_dec (qu,st,l)
           (NonFinal (ba,t,p,bl,bl2,e,h))
           (NonFinal (ba',t',p',bl',bl2',e',h')) <=>
@@ -78,7 +84,7 @@ val TRANSFER_EXCLUDED_dec_def = Define `
                 /\ (NULL ba) /\ (t = t') /\ (e = e') /\ (h = h') /\ (bl = bl') /\ F) /\
     (TRANSFER_EXCLUDED_dec _ (Final _) _ = F) /\
     (TRANSFER_EXCLUDED_dec _ _ (Final _) = F) `;
-
+*)
 
 val _ = export_theory ();
 
