ActVarRulesSpecScript.sml
@@ -55,7 +55,9 @@ val TRANSFER_def = Define `
            /\ (nbl = [])
            /\ (nba = FLAT (get_cand_pile_list bl p))
            /\ (!d. MEM d bl ==> (MEM (d,[]) np))
-           /\ (!d'. ((~ MEM d' bl) ==> (!l'. (MEM (d',l') p ==> MEM (d',l') np) /\ (MEM (d',l') np ==> MEM (d',l') p)))))
+           /\ (!d'. ((~ MEM d' bl) ==> (!l'. (MEM (d',l') p ==> MEM (d',l') np)
+                            /\ (MEM (d',l') np ==> MEM (d',l') p)))))
+
            /\ (j2 = NonFinal (nba, t, np, nbl, nbl2, e, h))`;
 
 (* COUNT rule *)
@@ -71,7 +73,7 @@ val COUNT_def = Define `
                              ?(l': ((cand list) # rat) list).
                                (l' = FILTER (\ (b: (cand list) # rat). (first_continuing_cand c (FST b) h)) ba)
                             /\ (get_cand_pile c np = (get_cand_pile c p) ++ [l'])
-                            /\ (get_cand_tally c nt = (get_cand_tally c t) + (SUM_RAT (MAP SND l'))))
+                            /\ (get_cand_tally c nt = (get_cand_tally c t) + (SUM_RAT (l'))))
                             /\ (~ MEM c h ==>
                                            (get_cand_pile c np = get_cand_pile c p)
                                         /\ (get_cand_tally c nt = get_cand_tally c t))))
@@ -82,7 +84,7 @@ val ELECT_def = Define `
   ELECT ((qu,st,l):params) j1 j2 <=>
   (? ba nba t nt p np bl nbl bl2 nbl2 e ne h nh l1.
     (j1 = NonFinal (ba, t, p, bl, bl2, e, h))
-     /\ (ELECT_Auxiliary (qu,st,l) ba t p np bl nbl e ne h nh)
+     /\ (ELECT_Auxiliary (qu,st,l) ba t p np bl nbl e ne h nh l1)
      /\ (ba = []) /\ (nba = []) /\ (t = nt) /\ (bl2 = []) /\ (nbl2 = [])
      /\ (nbl =  bl ++ l1)
      /\ (!c. MEM c l1 ==> (!l'. MEM (c,l') np ==>
@@ -94,7 +96,12 @@ val ELECT_def = Define `
                             /\ (MAP SND (Flat_l') = update_cand_trans_val qu c t PileCand_c)))
      /\ (j2 = NonFinal (nba, nt, np, nbl, nbl2, ne, nh)))`;
 
+val TRANSFER_EXCLUDED_def = Define `
+    TRANSFER_EXCLUDED (qu,st,l) j1 j2 <=> TRANSFER_EXCLUDED_Auxiliary (qu,st,l) j1 j2`;
 
+
+
+(*
 val TRANSFER_EXCLUDED_def = Define `
     TRANSFER_EXCLUDED (qu,st,l) j1 j2 <=>
       (? ba nba t nt p np bl nbl bl2 nbl2 e ne h nh.
@@ -102,7 +109,7 @@ val TRANSFER_EXCLUDED_def = Define `
        /\ (TRANSFER_EXCLUDED_Auxiliary (qu,st,l) nba t p np bl2 nbl2 e h)
        /\ (ba = []) /\ (t = nt) /\ (e = ne) /\ (h = nh) /\ (bl = nbl)
        /\ (j2 = NonFinal (nba,nt,np,nbl,nbl2,ne,nh))) /\ F`;
-
+*)
 
 
 val _ = export_theory ();
